testing harmonic

SP1Chips/AddiChip.lean
@@ -10,61 +10,62 @@ open LeanRV64D.Functions BitVec
 namespace Addi
 
 variable
-  (Main : Vector (Fin BB) 30)
+  (Main : Vector (Fin BB) 31)
   (s : SailState)
-  (cstrs : (constraints Main).allHold)
-  (h_is_real : Main[29] = 1)
 
 noncomputable def spec_addi (imm : BitVec 12) (rs1 rd : regidx) : SailM Unit := do
   Sail.writeReg Register.nextPC ((← Sail.readReg Register.PC) + 4#64)
   _ ← execute_ITYPE imm rs1 rd iop.ADDI
   pure ()
 
-def sp1_op_a : BitVec 5 :=
-  by
-    refine BitVec.ofNatLT Main[6] ?_
-    simp
-    show Main[6] < 32
+def sp1_op_a : BitVec 5 := BitVec.ofNat 5 Main[6]
+  -- by
+  --   refine BitVec.ofNatLT Main[6] ?_
+  --   simp
+  --   show Main[6] < 32
 
-    have reader_cstrs := by
-      simp [SP1ConstraintList.allHold, constraints, SP1Constraint.toProp] at cstrs
-      exact cstrs.2.2.1
+  --   have reader_cstrs := by
+  --     simp [SP1ConstraintList.allHold, constraints, SP1Constraint.toProp] at cstrs
+  --     exact cstrs.2.2.1
 
-    clear cstrs
-    simp [ITypeReader.constraints, h_is_real, Opcode.ofNat, Nat.ble, Nat.beq, SP1Constraint.toProp] at reader_cstrs
+  --   clear cstrs
+  --   simp [ITypeReader.constraints, h_is_real, Opcode.ofNat, Nat.ble, Nat.beq, SP1Constraint.toProp] at reader_cstrs
+  --   simp_all
 
-    exact reader_cstrs.1.2.1
+  --   exact reader_cstrs.1.2.1
 
-def sp1_op_b : BitVec 5 :=
-  by
-    refine BitVec.ofNatLT Main[14] ?_
-    simp
-    show Main[14] < 32
+def sp1_op_b : BitVec 5 := BitVec.ofNat 5 Main[14]
+  -- by
+  --   refine BitVec.ofNatLT Main[14] ?_
+  --   simp
+  --   show Main[14] < 32
 
-    have reader_cstrs := by
-      simp [SP1ConstraintList.allHold, constraints, SP1Constraint.toProp] at cstrs
-      exact cstrs.2.2.1
+  --   have reader_cstrs := by
+  --     simp [SP1ConstraintList.allHold, constraints, SP1Constraint.toProp] at cstrs
+  --     exact cstrs.2.2.1
 
-    clear cstrs
-    simp [ITypeReader.constraints, h_is_real, Opcode.ofNat, Nat.ble, Nat.beq, SP1Constraint.toProp] at reader_cstrs
+  --   clear cstrs
+  --   simp [ITypeReader.constraints, h_is_real, Opcode.ofNat, Nat.ble, Nat.beq, SP1Constraint.toProp] at reader_cstrs
 
-    exact reader_cstrs.1.1.1
+  --   exact reader_cstrs.1.1.1
 
-def sp1_op_c : BitVec 12 := BitVec.ofNat 12 Main[21].val
+def sp1_op_c : BitVec 12 := BitVec.ofNat 12 Main[21]
 
 def sp1_addi : SailM Unit := do
-  let op_a := sp1_op_a Main cstrs h_is_real
+  let op_a := sp1_op_a Main ---cstrs h_is_real
   Sail.writeReg Register.nextPC (Word.toBitVec64 #v[Main[3] + 4, Main[4], Main[5], 0])
-  Sail.write_reg op_a (Word.toBitVec64 #v[Main[25], Main[26], Main[27], Main[28]])
+  Sail.write_reg op_a (Word.toBitVec64 #v[Main[26], Main[27], Main[28], Main[29]])
 
 open Sail
 
 theorem correct_addi
+  (cstrs : (constraints Main).allHold)
+  (h_is_real : Main[30] = 1)
   (state_cstrs : (constraints Main).initialState s) :
   let op_c := sp1_op_c Main
-  let op_b := sp1_op_b Main cstrs h_is_real
-  let op_a := sp1_op_a Main cstrs h_is_real
-  (spec_addi op_c (.Regidx op_b) (.Regidx op_a)).run s = (sp1_addi Main cstrs h_is_real).run s
+  let op_b := sp1_op_b Main --cstrs h_is_real
+  let op_a := sp1_op_a Main --cstrs h_is_real
+  (spec_addi op_c (.Regidx op_b) (.Regidx op_a)).run s = (sp1_addi Main).run s
   := by
     -- Obtain and simplify state and pure constraints
     simp [SP1ConstraintList.initialState, constraints, SP1Constraint.toStateProp, List.Forall, AddOperation.constraints, CPUState.constraints, ITypeReader.constraints, h_is_real] at state_cstrs
@@ -73,7 +74,39 @@ theorem correct_addi
     obtain ⟨add_op_cstrs, cpu_cstrs, reader_cstrs, rest⟩ := cstrs
     rw [CPUState.allHold_constraints_iff_is_real h_is_real] at cpu_cstrs
     rw [ITypeReader.allHold_constraints_iff_is_real h_is_real] at reader_cstrs
-    obtain ⟨ trusted_instr_prop, _, _, c0, c1, c2, c3, _, _, _, _, _, _, _, _, _, _, ⟨ is_U64_a, is_U64_b, _ ⟩⟩ := reader_cstrs
+
+    specialize read_op_b sorry
+    specialize read_op_c sorry
+
+    obtain ⟨ trusted_instr_prop, hcm1, hcm2, c0, c1, c2, c3, h11, h12, h13, h14, h15, h16, h17, h18, h19, h20, ⟨ is_U64_a, is_U64_b, hu64 ⟩⟩ := reader_cstrs
+
+    simp [Opcode.ofNat, Nat.ble] at trusted_instr_prop
+    simp only [BitVec.ofNatLT_eq_ofNat] at *
+    simp [spec_addi, sp1_addi, execute, execute_ITYPE]
+    have hs : s.isInitialized := sorry
+    simp [run_readReg_of_isInitialized _ _ hs]
+    simp [sp1_op_b, read_op_b]
+    simp [sp1_op_c, read_op_c]
+    simp [sp1_op_a]
+
+    by_cases h_is_op_a_0 : Main[6] = 0
+    · simp [h_is_op_a_0]
+      have : #v[Main[26], Main[27], Main[28], Main[29]] = 0 := by sorry
+      simp [this]
+      simp [Word.toBitVec64, Word.toNat]
+      refine congr_arg _ ?_
+
+      rw [Std.ExtDHashMap.get?_eq_some_get] at read_pc
+      simp at read_pc
+      rw [Std.ExtDHashMap.get?_eq_some_get] at read_pc
+      rw [read_pc]
+      erw [Option.some_inj] at read_pc
+      rw [BabyBear.add4_into_pc_ofNat (by omega)]
+      sorry
+    ·
+      sorry
+
+    stop
     simp_all [Opcode.ofNat, Nat.ble]
     have is_U64_c : Word.isU64 #v[Main[21], Main[22], Main[23], Main[24]]
       := by apply Word.isU64_of_cases c0 c1 c2 c3
@@ -82,7 +115,7 @@ theorem correct_addi
     apply AddOperation.spec is_U64_b is_U64_c at add_op_cstrs
     obtain ⟨ is_U64_val, is_add ⟩ := add_op_cstrs
     simp at *
-
+    simp [BitVec.ofNatLT_eq_ofNat] at *
     -- Now the monadic manipulation
     simp [spec_addi, sp1_addi, execute, execute_ITYPE]
     rw [run_readReg, read_pc]
@@ -91,12 +124,18 @@ theorem correct_addi
     simp [sp1_op_a]
     rw [BabyBear.add4_into_pc_ofNat (by omega)]
 
-    by_cases h_is_op_a_0 : Main[6] = 0 <;> simp_all
-    . rw [← is_add]
+    by_cases h_is_op_a_0 : Main[6] = 0
+    .
+      -- have h13 : Main[13] = 1 := by sorry
+      -- simp [h13, h_is_op_a_0, Opcode.ofNat, Nat.ble] at *
+      have : #v[Main[26], Main[27], Main[28], Main[29]] = 0 := by sorry
+      simp [h_is_op_a_0, this, Word.toBitVec64, Word.toNat]
+
+    . rw [if_neg (by sorry)]
+      rw [if_neg (by sorry)]
       simp [Word.toBitVec64, Word.toNat]
-    . rw [if_neg (by simpa [← BitVec.toNat_inj])]
-      rw [if_neg (by simpa [← BitVec.toNat_inj])]
-      simp [Word.toBitVec64, Word.toNat]
+      congr 2
+
       rfl
 
 end Addi
